Exposed missing stuff

code/ecdsap256/dist/Hacl_Kremlib.h
@@ -35,6 +35,8 @@
 
 static inline uint64_t FStar_UInt64_eq_mask(uint64_t a, uint64_t b);
 
+static inline uint8_t FStar_UInt8_eq_mask(uint8_t a, uint8_t b);
+
 static inline uint128_t FStar_UInt128_add(uint128_t a, uint128_t b);
 
 static inline uint128_t FStar_UInt128_shift_left(uint128_t a, uint32_t s);
