code/ecdsap256/dist/Hacl_P256.d
@@ -7,4 +7,5 @@
  kremlin/internal/fstar_int.h kremlin/internal/compat.h \
  kremlin/internal/FStar_UInt_8_16_32_64.h \
  kremlin/internal/LowStar_Endianness.h kremlin/lowstar_endianness.h \
- wnaf.h lib_intrinsics.h Hacl_Kremlib.h Hacl_Spec.h Hacl_Lib.h
+ wnaf.h lib_intrinsics.h Hacl_Kremlib.h Hacl_Hash_SHA2.h \
+ Hacl_Hash_Core_SHA2.h Hacl_Spec.h Hacl_Lib.h
