code/ecdsap256/dist/Hacl_P256.h
@@ -32,8 +32,269 @@
 
 
 #include "Hacl_Kremlib.h"
+#include "Hacl_Hash_SHA2.h"
 #include "Hacl_Spec.h"
 #include "Hacl_Lib.h"
+
+/*
+ Input: result buffer: uint8[64], 
+ m buffer: uint8 [mLen], 
+ priv(ate)Key: uint8[32], 
+ k (nonce): uint32[32]. 
+  
+ Output: bool, where True stands for the correct signature generation. False value means that an error has occurred. 
+  
+ The private key and the nonce are expected to be more than 0 and less than the curve order.
+*/
+bool
+Hacl_P256_ecdsa_sign_p256_sha2_ladder(
+  uint8_t *result,
+  uint32_t mLen,
+  uint8_t *m,
+  uint8_t *privKey,
+  uint8_t *k
+);
+
+/*
+ Input: result buffer: uint8[64], 
+ m buffer: uint8 [mLen], 
+ priv(ate)Key: uint8[32], 
+ k (nonce): uint32[32]. 
+  
+ Output: bool, where True stands for the correct signature generation. False value means that an error has occurred. 
+  
+ The private key and the nonce are expected to be more than 0 and less than the curve order.
+*/
+bool
+Hacl_P256_ecdsa_sign_p256_sha2_comb(
+  uint8_t *result,
+  uint32_t mLen,
+  uint8_t *m,
+  uint8_t *privKey,
+  uint8_t *k
+);
+
+/*
+ Input: result buffer: uint8[64], 
+ m buffer: uint8 [mLen], 
+ priv(ate)Key: uint8[32], 
+ k (nonce): uint32[32]. 
+  
+ Output: bool, where True stands for the correct signature generation. False value means that an error has occurred. 
+  
+ The private key and the nonce are expected to be more than 0 and less than the curve order.
+*/
+bool
+Hacl_P256_ecdsa_sign_p256_sha384(
+  uint8_t *result,
+  uint32_t mLen,
+  uint8_t *m,
+  uint8_t *privKey,
+  uint8_t *k
+);
+
+/*
+ Input: result buffer: uint8[64], 
+ m buffer: uint8 [mLen], 
+ priv(ate)Key: uint8[32], 
+ k (nonce): uint32[32]. 
+  
+ Output: bool, where True stands for the correct signature generation. False value means that an error has occurred. 
+  
+ The private key and the nonce are expected to be more than 0 and less than the curve order.
+*/
+bool
+Hacl_P256_ecdsa_sign_p256_sha512(
+  uint8_t *result,
+  uint32_t mLen,
+  uint8_t *m,
+  uint8_t *privKey,
+  uint8_t *k
+);
+
+/*
+ Input: result buffer: uint8[64], 
+ m buffer: uint8 [mLen], 
+ priv(ate)Key: uint8[32], 
+ k (nonce): uint32[32]. 
+  
+ Output: bool, where True stands for the correct signature generation. False value means that an error has occurred. 
+  
+ The private key and the nonce are expected to be more than 0 and less than the curve order.
+  
+ The message m is expected to be hashed by a strong hash function, the lenght of the message is expected to be 32 bytes and more.
+*/
+bool
+Hacl_P256_ecdsa_sign_p256_without_hash_ladder(
+  uint8_t *result,
+  uint32_t mLen,
+  uint8_t *m,
+  uint8_t *privKey,
+  uint8_t *k
+);
+
+/*
+ Input: result buffer: uint8[64], 
+ m buffer: uint8 [mLen], 
+ priv(ate)Key: uint8[32], 
+ k (nonce): uint32[32]. 
+  
+ Output: bool, where True stands for the correct signature generation. False value means that an error has occurred. 
+  
+ The private key and the nonce are expected to be more than 0 and less than the curve order.
+  
+ The message m is expected to be hashed by a strong hash function, the lenght of the message is expected to be 32 bytes and more.
+*/
+bool
+Hacl_P256_ecdsa_sign_p256_without_hash_comb(
+  uint8_t *result,
+  uint32_t mLen,
+  uint8_t *m,
+  uint8_t *privKey,
+  uint8_t *k
+);
+
+/*
+ The input of the function is considered to be public, 
+  thus this code is not secret independent with respect to the operations done over the input.
+  
+ Input: m buffer: uint8 [mLen], 
+ pub(lic)Key: uint8[64], 
+ r: uint8[32], 
+ s: uint8[32]. 
+  
+ Output: bool, where true stands for the correct signature verification. 
+*/
+bool
+Hacl_P256_ecdsa_verif_p256_sha2_ladder(
+  uint32_t mLen,
+  uint8_t *m,
+  uint8_t *pubKey,
+  uint8_t *r,
+  uint8_t *s
+);
+
+/*
+ The input of the function is considered to be public, 
+  thus this code is not secret independent with respect to the operations done over the input.
+  
+ Input: m buffer: uint8 [mLen], 
+ pub(lic)Key: uint8[64], 
+ r: uint8[32], 
+ s: uint8[32]. 
+  
+ Output: bool, where true stands for the correct signature verification. 
+*/
+bool
+Hacl_P256_ecdsa_verif_p256_sha2_comb_radix(
+  uint32_t mLen,
+  uint8_t *m,
+  uint8_t *pubKey,
+  uint8_t *r,
+  uint8_t *s
+);
+
+/*
+ The input of the function is considered to be public, 
+  thus this code is not secret independent with respect to the operations done over the input.
+  
+ Input: m buffer: uint8 [mLen], 
+ pub(lic)Key: uint8[64], 
+ r: uint8[32], 
+ s: uint8[32]. 
+  
+ Output: bool, where true stands for the correct signature verification.
+  
+ The message m is expected to be hashed by a strong hash function, the lenght of the message is expected to be 32 bytes and more.
+*/
+bool
+Hacl_P256_ecdsa_verif_without_hash_ladder(
+  uint32_t mLen,
+  uint8_t *m,
+  uint8_t *pubKey,
+  uint8_t *r,
+  uint8_t *s
+);
+
+/*
+ The input of the function is considered to be public, 
+  thus this code is not secret independent with respect to the operations done over the input.
+  
+ Input: m buffer: uint8 [mLen], 
+ pub(lic)Key: uint8[64], 
+ r: uint8[32], 
+ s: uint8[32]. 
+  
+ Output: bool, where true stands for the correct signature verification.
+  
+ The message m is expected to be hashed by a strong hash function, the lenght of the message is expected to be 32 bytes and more.
+*/
+bool
+Hacl_P256_ecdsa_verif_without_hash_comb(
+  uint32_t mLen,
+  uint8_t *m,
+  uint8_t *pubKey,
+  uint8_t *r,
+  uint8_t *s
+);
+
+/*
+ Public key verification function. 
+  
+  The input of the function is considered to be public, 
+  thus this code is not secret independent with respect to the operations done over the input.
+  
+ Input: pub(lic)Key: uint8[64]. 
+  
+ Output: bool, where 0 stands for the public key to be correct with respect to SP 800-56A:  
+ Verify that the public key is not the “point at infinity”, represented as O. 
+ Verify that the affine x and y coordinates of the point represented by the public key are in the range [0, p – 1] where p is the prime defining the finite field. 
+ Verify that y2 = x3 + ax + b where a and b are the coefficients of the curve equation. 
+ Verify that nQ = O (the point at infinity), where n is the order of the curve and Q is the public key point.
+  
+ The last extract is taken from : https://neilmadden.blog/2017/05/17/so-how-do-you-validate-nist-ecdh-public-keys/
+*/
+bool Hacl_P256_verify_q(uint8_t *pubKey);
+
+/*
+ There and further we introduce notions of compressed point and not compressed point. 
+  
+ We denote || as byte concatenation. 
+  
+ A compressed point is a point representaion as follows: (0x2 + y % 2) || x.
+  
+ A not Compressed point is a point representation as follows: 0x4 || x || y.
+
+  
+ 
+ Input: a point in not compressed form (uint8[65]), 
+ result: uint8[64] (internal point representation).
+  
+ Output: bool, where true stands for the correct decompression.
+ 
+*/
+bool Hacl_P256_decompression_not_compressed_form(uint8_t *b, uint8_t *result);
+
+/*
+ Input: a point in compressed form (uint8[33]), 
+ result: uint8[64] (internal point representation).
+  
+ Output: bool, where true stands for the correct decompression.
+ 
+*/
+bool Hacl_P256_decompression_compressed_form(uint8_t *b, uint8_t *result);
+
+/*
+ Input: a point buffer (internal representation: uint8[64]), 
+ result: a point in not compressed form (uint8[65]).
+*/
+void Hacl_P256_compression_not_compressed_form(uint8_t *b, uint8_t *result);
+
+/*
+ Input: a point buffer (internal representation: uint8[64]), 
+ result: a point in not compressed form (uint8[33]).
+*/
+void Hacl_P256_compression_compressed_form(uint8_t *b, uint8_t *result);
 
 /*
  Input: result: uint8[64], 
